\documentclass[12pt, a4paper]{article}

\usepackage{geometry}
\usepackage{amsmath}
\usepackage{amssymb}
\usepackage{fancyhdr}
\usepackage{pgfplots}
\usepackage{cancel}
\usepackage{scalerel}
\usepgfplotslibrary{fillbetween}
\usepackage{comment}

\setlength{\headheight}{50pt}
\addtolength{\topmargin}{-29.68335pt}
\pgfplotsset{
    compat=1.18,
    standard/.style={
    font=\tiny,
    axis line style = thick,
    trig format=rad,
    enlargelimits,
    axis x line=middle,
    axis y line=middle,
    enlarge x limits=0.00005,
    enlarge y limits=0.00005,
    every axis x label/.style={at={(ticklabel* cs:1.05)},anchor=north west},
    every axis y label/.style={at={(ticklabel* cs:1.05)},anchor=south east}
    }
}

\pagestyle{fancy}
\renewcommand{\headrulewidth}{0pt}
\renewcommand{\footrulewidth}{0pt}

\author{Kalle Alkula}
\title{Calculus.vk38}
\date\today
\fancyhf{}
\rhead{
    PINFOSS 22\\
    Kalle.alkula@turkuamk.fi
}
\rfoot{page \thepage}
\begin{document}
\maketitle
\thispagestyle{fancy}
    \paragraph*{18.}
        \textit{
            \\
            \textbf{a)}
        }
    \begin{equation*}
        \begin{split}
        f(x) &=\sqrt{x}\\\\
        f'(x) &= D[~\sqrt{1}~]\\
        &=\frac{1}{2\sqrt{1}}\\
        &= \frac{1}{2}\\
        \end{split}
    \end{equation*}
    \textit{
        \textbf{b)}
    }
    \begin{equation*}
        \begin{split}
            f(x)&= 4\sqrt[3]{x}\\\\
            f'(x)&= D[~4~]~D[~\sqrt[3]{2}~]\\
            &= \frac{1}{3\sqrt[3]{2^2}}\\
        \end{split}
    \end{equation*}
    \newpage
    \paragraph*{25.}
        \textit{
            \\
            \textbf{a)}
        }
    \begin{equation*}
        \begin{split}
            a(x)&= x cos(x)\\\\
            a'(x)&= D[x]~cos(x) + x~D[cos(x)]\\
            &= cos(x) -xsin(x)\\
        \end{split}
    \end{equation*}
        \textit{
            \textbf{b)}
        }
        \begin{equation*}
            \begin{split}
                b(x)&=\frac{2x}{x+3}\\\\
                b'(x)&=\frac{2x}{x+3}\\
                &=\frac{D[~2x~]x+3 -2xD[~x+3~]}{(x+3)^2}\\
                &=\frac{2x+6 -2x}{(x+3)^2}\\
                &=\frac{6}{(x+3)^2}\\
            \end{split}
        \end{equation*}
        \textit{
            \textbf{c)}
        }
        \begin{equation*}
            \begin{split}
                c(x)&= x^2 IN x\\\\
                c'(x)&= x^2 IN x\\
                &=D[~x^2~] IN x + x^2 D[~IN x~]\\
                &=2xIn x + x\\
            \end{split}
        \end{equation*}
        \textit{
            \textbf{d)}
        }
        \begin{equation*}
            \begin{split}
                d(x)&= \frac{sin(x)}{x}\\\\\\
                d'(x)&= \frac{sin(x)}{x}\\\\
                &=\frac{D[sinx(x)] x -sin(x) D[~x~]}{x^2}\\
                &=\frac{xcos(x)-sin(x)}{x^2}\\
            \end{split}
        \end{equation*}
        \newpage
        \paragraph*{26.}
        \textit{
            \\
            \textbf{a)}
        }
        \begin{equation*}
            \begin{split}
                a(x)&= 2x sin(3x)\\\\
                a'(x)&= 2x sin(3x)\\
                &= D[~2x~]sin(3x)+ 2x D[sin(3x)]\\
                &= 2sin(3x) + 6xcos(3x)\\
            \end{split}
        \end{equation*}
        \textit{
            \textbf{b)}
        }
        \begin{equation*}
            \begin{split}
                b(x)&= \frac{x^2}{sin(x)}\\\\
                b'(x)&= \frac{D[~x^2~]sin(x)- x^2 D[sin(x)]}{sin^2(x)}\\
                &= \frac{2xsin(x)-x^2cos(x)}{sin^2(x)}\\
            \end{split}
        \end{equation*}
        \textit{
            \textbf{c)}
        }
        \begin{equation*}
            \begin{split}
                c(x)&= 3x^2 e^{2x}\\\\
                c'(x)&= D[~3x^2~]e^{2x}+ 3x^2 D[~e^{2x}~]\\
                &=6xe^{2x}+6x^2e^{2x}\\
                &=6xe^2(x+x^2)\\
            \end{split}
        \end{equation*}
        \textit{
            \textbf{d)}
        }
        \begin{equation*}
            \begin{split}
                d(x)&= \frac{x}{2x^2+1}\\\\
                d'(x)&=\frac{D[~x~]2x^2+1 -x~D[~2x^2+1~]}{(2x^2 + 1)^2}\\
                &=\frac{1-2x^2-4x^2}{(2x^2+1)^2}\\
                &=\frac{1-2x^2}{(2x^2+1)^2}\\
            \end{split}
        \end{equation*}
        \newpage
        \paragraph{23.}
        \textit{
            \\
            \textbf{a)}
        }
        \begin{equation*}
            \begin{split}
                f(x)&= e^{5x}\\\\
                f'(x)&= D[e^{5x}]~~D[~5x~]\\
                &=5e^{5x}\\
            \end{split}
        \end{equation*}
        \textit{
            \textbf{b)}
        }
        \begin{equation*}
            \begin{split}
                f(x)&= sin(100x+0,1)\\\\
                f'(x)&= D[sin(100x+0,1)]\\
                &= 100cos(100x+0,1)\\
            \end{split}
        \end{equation*}
        \textit{
            \textbf{c)}
        }
        \begin{equation*}
            \begin{split}
                f(x)&=e^{-x^2}\\\\
                f'(x)&=D[~e^{-x^2}~]~~D[~-x^2~]\\
                &=-2xe^{-x^2}\\
            \end{split}
        \end{equation*}
        \textit{
            \textbf{d)}
        }
        \begin{equation*}
            \begin{split}
                n(t)&= 3e^{-2t}-2e^{-5t}\\\\
                n'(t)&= D[~3e^{-2t}~] -2e^{-5t}+3e^{-2t}D[~-2e^{-5t}~]\\
                &=-6e^{-2t}+ 10e^{-5t}\\
            \end{split}
        \end{equation*}
        \textit{
            \textbf{e)}
        }
        \begin{equation*}
            \begin{split}
                f(t)&=3sin(4t)-7cos(4t)\\\\
                f'(t)&=D[~3sin(4t)~]~D[~-7cos(4t)~]\\
                &=12cos(4t)-28sin(4t)\\
            \end{split}
        \end{equation*}
        \newpage
        \paragraph*{27.}
        \textit{
            \\
            \textbf{a)}
        }
        \begin{equation*}
            \begin{split}
                y&=(3x^2 +1)^4\\\\
                y'&=D[~3x^2+1~]~D[u^4]\\
                &=24x(3x^2+1)^3\\
            \end{split}
        \end{equation*}
        \textit{
            \textbf{b)}
        }
        \begin{equation*}
            \begin{split}
                y&=sin^3x\\\\
                y'&=D[~sinx~] D[~u^3~]\\
                &= 3sin^2 + cos^3x\\
            \end{split}
        \end{equation*}
        \textit{
            \textbf{c)}
        }
        \begin{equation*}
            \begin{split}
                y&=\sqrt{5x^2+2}\\\\
                y'&=D[\sqrt{5x^2+2}]~D[5x^2+2]\\
                &=10x\frac{1}{2\sqrt{5x^2+2}}\\
                &=\frac{2\times 5x}{2\sqrt{5x^2+2}}\\
                &=\frac{5x}{\sqrt{5x^2+2}}\\
            \end{split}
        \end{equation*}






\end{document}